src/asn1/ASN1.Spec.TLV.fst
@@ -183,3 +183,8 @@ let length_of_TLV
 
 let _ =
 assert_norm (length_of_asn1_primitive_value (Mkbit_string_t 33ul 1ul (magic())) == 33)
+
+#push-options "--z3rlimit 32"
+let _ =
+  lemma_serialize_asn1_oid_TLV_size OID_RIOT;
+assert (length_of_asn1_primitive_TLV OID_RIOT == 11)
