src/asn1/RIoT.X509.CompositeDeviceID.fst
@@ -7,7 +7,7 @@ open ASN1.Spec
 open ASN1.Low
 
 open X509.Base
-open X509.BasicFields
+open X509.BasicFields.SubjectPublicKeyInfo
 open X509.Crypto
 open RIoT.X509.Base
 open RIoT.X509.FWID
@@ -115,39 +115,20 @@ let lemma_serialize_compositeDeviceID_unfold
     // lemma_serialize_fwid_sequence_TLV_unfold x.riot_fwid;
     // lemma_serialize_fwid_unfold              x.riot_fwid
 
-#push-options "--query_stats --z3rlimit 32"
 let lemma_serialize_compositeDeviceID_size
   (x: compositeDeviceID_t)
 : Lemma (
   length_of_opaque_serialization (serialize_compositeDeviceID) x ==
   length_of_asn1_primitive_TLV x.riot_version +
   length_of_opaque_serialization (serialize_subjectPublicKeyInfo_sequence_TLV alg_DeviceID) x.riot_deviceID +
-  length_of_opaque_serialization serialize_fwid_sequence_TLV x.riot_fwid
-  // (* subjectPublicKeyInfo size *)
-  // length_of_opaque_serialization (serialize_subjectPublicKeyInfo alg_DeviceID) x.riot_deviceID ==
-  // length_of_asn1_sequence_TLV (serialize_algorithmIdentifier alg_DeviceID) x.riot_deviceID.subjectPubKey_alg +
-  // length_of_asn1_primitive_TLV x.riot_deviceID.subjectPubKey /\
-  // (* algorithmIdentifier size*)
-  // ( match alg_DeviceID with
-  //   | ECDSA_P256 -> length_of_opaque_serialization (serialize_algorithmIdentifier alg_DeviceID) x.riot_deviceID.subjectPubKey_alg ==
-  //                   length_of_asn1_primitive_TLV x.riot_deviceID.subjectPubKey_alg.alg_id_oid_ecdsa +
-  //                   length_of_asn1_primitive_TLV x.riot_deviceID.subjectPubKey_alg.alg_id_oid_p256 ) /\
-  // (* FWID size *)
-  // length_of_opaque_serialization serialize_fwid x.riot_fwid ==
-  // length_of_asn1_primitive_TLV x.riot_fwid.fwid_hashAlg +
-  // length_of_asn1_primitive_TLV x.riot_fwid.fwid_value
+  length_of_opaque_serialization serialize_fwid_sequence_TLV x.riot_fwid /\
+  length_of_opaque_serialization serialize_compositeDeviceID x ==
+  length_of_asn1_primitive_TLV x.riot_version + 91 /\
+  length_of_opaque_serialization serialize_compositeDeviceID x <= 97
 )
-= lemma_serialize_compositeDeviceID_unfold x
-    // lemma_serialize_subjectPublicKeyInfo_sequence_TLV_unfold alg_DeviceID x.riot_deviceID;
-    // lemma_serialize_subjectPublicKeyInfo_sequence_TLV_size   alg_DeviceID x.riot_deviceID;
-    // lemma_serialize_subjectPublicKeyInfo_unfold              alg_DeviceID x.riot_deviceID;
-    // lemma_serialize_subjectPublicKeyInfo_size                alg_DeviceID x.riot_deviceID;
-    //   lemma_serialize_algorithmIdentifier_sequence_TLV_unfold alg_DeviceID x.riot_deviceID.subjectPubKey_alg;
-    //   lemma_serialize_algorithmIdentifier_sequence_TLV_size   alg_DeviceID x.riot_deviceID.subjectPubKey_alg;
-    //   lemma_serialize_algorithmIdentifier_size                alg_DeviceID x.riot_deviceID.subjectPubKey_alg;
-    // lemma_serialize_fwid_sequence_TLV_unfold x.riot_fwid;
-    // lemma_serialize_fwid_sequence_TLV_size   x.riot_fwid;
-    // lemma_serialize_fwid_size                x.riot_fwid
+= lemma_serialize_compositeDeviceID_unfold x;
+    lemma_serialize_subjectPublicKeyInfo_sequence_TLV_size_exact alg_DeviceID x.riot_deviceID;
+    lemma_serialize_fwid_sequence_TLV_size_exact x.riot_fwid
 
 (* inbound sub type*)
 let compositeDeviceID_t_inbound
@@ -178,13 +159,23 @@ let lemma_serialize_compositeDeviceID_sequence_TLV_size
 : Lemma ( prop_serialize_asn1_sequence_TLV_size serialize_compositeDeviceID x )
 = lemma_serialize_asn1_sequence_TLV_size serialize_compositeDeviceID x
 
+open FStar.Integers
+#push-options "--z3rlimit 32 --fuel 4 --ifuel 4"
 let lemma_serialize_compositeDeviceID_sequence_TLV_size_exact
   (x: compositeDeviceID_t_inbound)
 : Lemma (
-  length_of_opaque_serialization serialize_compositeDeviceID x ==
-  length_of_asn1_primitive_TLV x.riot_version + 93
+  length_of_opaque_serialization serialize_compositeDeviceID_sequence_TLV x ==
+  length_of_asn1_primitive_TLV x.riot_version + 93 /\
+  length_of_opaque_serialization serialize_compositeDeviceID_sequence_TLV x <= 99
 )
-= admit()//lemma_serialize_asn1_sequence_TLV_size serialize_compositeDeviceID x
+= lemma_serialize_compositeDeviceID_sequence_TLV_unfold x;
+  lemma_serialize_compositeDeviceID_sequence_TLV_size   x;
+    lemma_serialize_compositeDeviceID_size x;
+    assert (length_of_opaque_serialization serialize_compositeDeviceID_sequence_TLV x ==
+            1 +
+            length_of_asn1_length (u (length_of_opaque_serialization serialize_compositeDeviceID x)) +
+            length_of_opaque_serialization serialize_compositeDeviceID x)
+#pop-options
 
 let serialize32_compositeDeviceID
 : serializer32_backwards (serialize_compositeDeviceID)
